Until while_dec

plf/Hoare2.v
@@ -10,3 +10,168 @@ From PLF Require Export Imp.
 From PLF Require Import Hoare.
 Set Default Goal Selector "!".
 Definition FILL_IN_HERE := <{True}>.
+
+(*
+  {{ True }}
+    if X <= Y then
+              {{ True /\ (X <= Y) }} ->>
+              {{ Y = X + (Y - X) }}
+      Z := Y - X
+              {{ Y = X + Z }}
+    else
+              {{ True /\ ~(X <= Y) }} ->>
+              {{ X + Z = X + Z }}
+      Y := X + Z
+              {{ Y = X + Z }}
+    end
+  {{ Y = X + Z }}
+*)
+
+Definition reduce_to_zero' : com :=
+  <{ while X <> 0 do
+        X := X - 1
+     end }>.
+
+Theorem reduce_to_zero_correct' :
+  {{True}}
+    reduce_to_zero'
+  {{X = 0}}.
+Proof.
+  unfold reduce_to_zero'.
+  eapply hoare_consequence_post.
+  - apply hoare_while.
+    + eapply hoare_consequence_pre.
+      * apply hoare_asgn.
+      * unfold assn_sub, "->>". simpl. intros.
+        exact I.
+  - intros st [Inv GuardFalse].
+    unfold bassn in GuardFalse. simpl in GuardFalse.
+    rewrite not_true_iff_false in GuardFalse.
+    rewrite negb_false_iff in GuardFalse.
+    apply eqb_eq in GuardFalse.
+    apply GuardFalse.
+Qed.
+
+Ltac verify_assn :=
+  repeat split;
+  simpl;
+  unfold assert_implies;
+  unfold ap in *; unfold ap2 in *;
+  unfold bassn in *; unfold beval in *; unfold aeval in *;
+  unfold assn_sub; intros;
+  repeat (simpl in *;
+          rewrite t_update_eq ||
+          (try rewrite t_update_neq;
+          [| (intro X; inversion X; fail)]));
+  simpl in *;
+  repeat match goal with [H : _ /\ _ |- _] =>
+                         destruct H end;
+  repeat rewrite not_true_iff_false in *;
+  repeat rewrite not_false_iff_true in *;
+  repeat rewrite negb_true_iff in *;
+  repeat rewrite negb_false_iff in *;
+  repeat rewrite eqb_eq in *;
+  repeat rewrite eqb_neq in *;
+  repeat rewrite leb_iff in *;
+  repeat rewrite leb_iff_conv in *;
+  try subst;
+  simpl in *;
+  repeat
+    match goal with
+      [st : state |- _] =>
+        match goal with
+        | [H : st _ = _ |- _] =>
+            rewrite -> H in *; clear H
+        | [H : _ = st _ |- _] =>
+            rewrite <- H in *; clear H
+        end
+    end;
+  try eauto;
+  try lia.
+
+Theorem reduce_to_zero_correct''' :
+  {{True}}
+    reduce_to_zero'
+  {{X = 0}}.
+Proof.
+  unfold reduce_to_zero'.
+  eapply hoare_consequence_post.
+  - apply hoare_while.
+    + eapply hoare_consequence_pre.
+      * apply hoare_asgn.
+      * verify_assn.
+  - verify_assn.
+Qed.
+
+Inductive dcom : Type :=
+| DCSkip (Q : Assertion)
+  (* skip {{ Q }} *)
+| DCSeq (d1 d2 : dcom)
+  (* d1 ; d2 *)
+| DCAsgn (X : string) (a : aexp) (Q : Assertion)
+  (* X := a {{ Q }} *)
+| DCIf (b : bexp) (P1 : Assertion) (d1 : dcom)
+       (P2 : Assertion) (d2 : dcom) (Q : Assertion)
+  (* if b then {{ P1 }} d1 else {{ P2 }} d2 end {{ Q }} *)
+| DCWhile (b : bexp) (P : Assertion) (d : dcom)
+          (Q : Assertion)
+  (* while b do {{ P }} d end {{ Q }} *)
+| DCPre (P : Assertion) (d : dcom)
+  (* ->> {{ P }} d *)
+| DCPost (d : dcom) (Q : Assertion)
+  (* d ->> {{ Q }} *).
+  
+Inductive decorated : Type :=
+  | Decorated : Assertion -> dcom -> decorated.
+  
+Declare Scope dcom_scope.
+Notation "'skip' {{ P }}"
+      := (DCSkip P)
+      (in custom com at level 0, P constr) : dcom_scope.
+Notation "l ':=' a {{ P }}"
+      := (DCAsgn l a P)
+      (in custom com at level 0, l constr at level 0,
+          a custom com at level 85, P constr, no associativity) : dcom_scope.
+Notation "'while' b 'do' {{ Pbody }} d 'end' {{ Ppost }}"
+      := (DCWhile b Pbody d Ppost)
+           (in custom com at level 89, b custom com at level 99,
+           Pbody constr, Ppost constr) : dcom_scope.
+Notation "'if' b 'then' {{ P }} d 'else' {{ P' }} d' 'end' {{ Q }}"
+      := (DCIf b P d P' d' Q)
+           (in custom com at level 89, b custom com at level 99,
+               P constr, P' constr, Q constr) : dcom_scope.
+Notation "'->>' {{ P }} d"
+      := (DCPre P d)
+      (in custom com at level 12, right associativity, P constr) : dcom_scope.
+Notation "d '->>' {{ P }}"
+      := (DCPost d P)
+      (in custom com at level 10, right associativity, P constr) : dcom_scope.
+Notation " d ; d' "
+      := (DCSeq d d')
+      (in custom com at level 90, right associativity) : dcom_scope.
+Notation "{{ P }} d"
+      := (Decorated P d)
+      (in custom com at level 91, P constr) : dcom_scope.
+Local Open Scope dcom_scope.
+Example dec0 :=
+  <{ skip {{ True }} }>.
+Example dec1 :=
+  <{ while true do {{ True }} skip {{ True }} end
+  {{ True }} }>.
+  
+Set Printing All.
+Print dec1.
+Unset Printing All.
+
+Example dec_while : decorated :=
+  <{
+    {{ True }}
+      while X <> 0
+      do
+                {{ True /\ ( X <> 0) }}
+        X := X - 1
+                {{ True }}
+      end
+    {{ True /\ X = 0 }} ->> {{ X = 0 }}
+  }>.
+  
